in progress: modules for hindsight

templates/hindsight/data_structure.v
@@ -49,3 +49,481 @@ Module Type DATA_STRUCTURE.
   Parameter Op_inhabited : Inhabited Op.
   
 End DATA_STRUCTURE.  
+
+Module HINDSIGHT_DEFS (DS : DATA_STRUCTURE).
+  Import DS.
+  
+  Global Instance snapshotUR_discrete' : CmraDiscrete snapshotUR.
+  Proof.
+    apply snapshotUR_discrete.
+  Qed.
+  
+  Global Instance absTUR_discrete' : CmraDiscrete absTUR.
+  Proof.
+    apply absTUR_discrete.
+  Qed.
+
+  Global Instance snapshot_leibnizequiv' : LeibnizEquiv (snapshot).
+  Proof.
+    apply snapshot_leibnizequiv.
+  Qed.  
+
+  Global Instance snapshot_inhabited' : Inhabited snapshot.
+  Proof.
+    apply snapshot_inhabited.
+  Qed.
+
+  Global Instance resT_inhabited' : Inhabited resT.
+  Proof.
+    apply resT_inhabited.
+  Qed.
+
+  Global Instance Op_inhabited' : Inhabited Op.
+  Proof.
+    apply Op_inhabited.
+  Qed.
+
+  
+  (* RAs used in proof *)
+
+  Definition auth_natUR := authUR $ max_natUR.
+  Definition agree_snapshotR := agreeR $ snapshotUR.
+  Definition frac_absTR := dfrac_agreeR $ absTUR.
+  Definition historyR := gmapUR nat $ snapshotUR.
+  Definition auth_historyR := authR $ gmapUR nat $ agree_snapshotR.
+  Definition frac_historyR := dfrac_agreeR $ historyR.
+  Definition tokenUR := exclR unitO.
+  Definition set_tidR := authR (gsetUR proph_id). 
+  Definition thread_viewR := authUR $ 
+                              gmapUR proph_id $ 
+                                agreeR $ prodO natO gnameO.
+
+  Class dsG Σ := DS {
+                  dsG_auth_natG :> inG Σ auth_natUR;
+                  dsG_agree_snapshotG :> inG Σ agree_snapshotR;
+                  dsG_frac_absTG :> inG Σ frac_absTR;
+                  dsG_historyG :> inG Σ historyR;
+                  dsG_auth_historyG :> inG Σ auth_historyR;
+                  dsG_tokenG :> inG Σ tokenUR;
+                  dsG_frac_historyG :> inG Σ frac_historyR;
+                  dsG_set_tidG :> inG Σ set_tidR;
+                  dsG_thread_viewG :> inG Σ thread_viewR
+                 }.
+                 
+  Definition dsΣ : gFunctors :=
+    #[ GFunctor auth_natUR; GFunctor agree_snapshotR;
+       GFunctor frac_absTR; GFunctor historyR;
+       GFunctor auth_historyR; GFunctor tokenUR; 
+       GFunctor frac_historyR; GFunctor set_tidR;
+       GFunctor thread_viewR ].
+  
+  Global Instance subG_dsΣ {Σ} : subG dsΣ Σ → dsG Σ.
+  Proof. solve_inG. Qed.
+
+  Context {Σ} `{!heapGS Σ, !dsG Σ}.
+  Notation iProp := (iProp Σ).
+  Implicit Types M : gmap nat snapshot.
+  Implicit Types T : nat.
+  
+  Global Definition cntrN N := N .@ "cntr".
+  Global Definition threadN N := N .@ "thread".
+  
+
+  Definition map_max (M: gmap nat snapshot) : nat := 
+    max_list (elements (dom M)).
+
+  Definition hist γ_t γ_m M T : iProp :=
+    ∃ (M': gmap nat (agreeR (_))),
+      own γ_t (● MaxNat T) ∗ own γ_m (● M')
+    ∗ ⌜T = map_max M⌝
+    ∗ ⌜map_Forall (λ k a, a = to_agree (M !!! k)) M'⌝
+    ∗ ⌜∀ t, t < T → M !!! t ≠ M !!! (t+1)%nat⌝.
+
+  Definition dsRep γ_s (a: absTUR) : iProp := 
+    own γ_s (to_frac_agree (1/2) a).
+
+  Definition dsRepI γ_s (a: absTUR) : iProp := 
+    own γ_s (to_frac_agree (1/2) a).
+    
+  (** Helping Inv **)
+  
+  Definition au N γ_r op (Q : val → iProp) := 
+    (AU << ∃∃ a, dsRep γ_r a >> 
+          @ ⊤ ∖ ↑(cntrN N), ∅
+        << ∀∀ a' res, dsRep γ_r a' ∗ ⌜seq_spec op a a' res⌝, COMM Q #res >>)%I.
+        
+  Definition past_lin M T op res t0 : iProp :=
+    ⌜match updater_thread op res with
+    | true =>
+      ∃ t, t0 ≤ t < T ∧ seq_spec op (abs (M !!! t)) (abs (M !!! (t+1)%nat)) res
+    | false =>  
+      ∃ t, t0 ≤ t ≤ T ∧ seq_spec op (abs (M !!! t)) (abs (M !!! t)) res end⌝.
+
+  Definition past_state γ_m (t0: nat) (s: snapshot) : iProp :=
+    ∃ t, ⌜t0 ≤ t⌝ ∗ own γ_m (◯ {[t := to_agree s]}).
+  
+  Definition past_two_states γ_m (t0: nat) (s s': snapshot) : iProp :=
+    ∃ t, ⌜t0 ≤ t⌝ 
+    ∗ own γ_m (◯ {[t := to_agree s]}) 
+    ∗ own γ_m (◯ {[t+1 := to_agree s']}).
+
+  Definition past_lin_witness γ_m op res t0 : iProp :=
+    match updater_thread op res with
+    | true =>
+      ∃ s s', past_two_states γ_m t0 s s' ∗ ⌜seq_spec op (abs s) (abs s') res⌝
+    | false =>  
+      ∃ s, past_state γ_m t0 s ∗ ⌜seq_spec op (abs s) (abs s) res⌝ end.
+
+  Definition Pending (P: iProp) M T op vp t0 : iProp := 
+    P ∗ £1 ∗ ¬ past_lin M T op vp t0.
+
+  Definition Done γ_tk (Q: val → iProp) M T op (vp: resT) t0 : iProp := 
+      (Q #vp ∨ own γ_tk (Excl ())) ∗ past_lin M T op vp t0.
+
+  Definition State γ_sy γ_tk P Q M T op vp t0 : iProp :=
+      own γ_sy (to_frac_agree (1/2) M)
+    ∗ ⌜T = map_max M⌝ 
+    ∗ (Pending P M T op vp t0 ∨ Done γ_tk Q M T op vp t0).
+
+  Definition thread_vars γ_t γ_ght γ_sy t_id t0 : iProp := 
+    own γ_ght (◯ {[t_id := to_agree (t0, γ_sy)]}) ∗ own γ_t (◯ MaxNat t0).
+
+  Definition Reg N γ_t γ_s γ_ght t_id M : iProp :=
+    ∃ γ_tk γ_sy Q op vp t0 (vtid: val), 
+        proph1 t_id vtid
+      ∗ thread_vars γ_t γ_ght γ_sy t_id t0
+      ∗ own (γ_sy) (to_frac_agree (1/2) M)
+      ∗ inv (threadN N) (∃ M T, State γ_sy γ_tk (au N γ_s op Q) Q M T op vp t0).
+
+  Definition helping_inv (N: namespace) γ_t γ_s γ_td γ_ght M : iProp :=
+    ∃ (R: gset proph_id) (hγt: gmap proph_id (agreeR _)),
+        own γ_td (● R)
+      ∗ own γ_ght (● hγt) ∗ ⌜dom hγt = R⌝  
+      ∗ ([∗ set] t_id ∈ R, Reg N γ_t γ_s γ_ght t_id M).
+  
+  Definition ds_inv N γ_t γ_s γ_m γ_td γ_ght template_inv : iProp :=
+    inv (cntrN N)
+    (∃ M T (s: snapshot),
+      dsRepI γ_s (abs s) ∗ ⌜abs (M !!! T) = abs s⌝
+    ∗ hist γ_t γ_m M T
+    ∗ helping_inv N γ_t γ_s γ_td γ_ght M
+    ∗ template_inv M T s).
+(*    
+  Instance dsRep_timeless : ∀ γ_s C, Timeless (dsRep γ_s C).
+  Proof.
+    intros γ_s C. rewrite /dsRep. Search Timeless. 
+    apply own_timeless; apply _.
+  Qed.   
+*)    
+  Definition update_helping_protocol N γ_t γ_s γ_td γ_ght : iProp :=
+        ∀ M T n s, 
+          ⌜map_max M = T⌝ -∗   
+            dsRep γ_s n -∗ own γ_t (● MaxNat T) -∗ 
+              helping_inv N γ_t γ_s γ_td γ_ght M ={⊤ ∖ ↑cntrN N}=∗
+                helping_inv N γ_t γ_s γ_td γ_ght (<[T := s]> M) 
+                ∗ dsRep γ_s n ∗ own γ_t (● MaxNat T).
+    
+End HINDSIGHT_DEFS.
+
+Module Type HINDSIGHT_SPEC (DS : DATA_STRUCTURE).
+  Module DEFS := HINDSIGHT_DEFS DS.
+  Import DEFS DS.
+
+  Parameter dsOp_spec: ∀ N γ_s γ_t γ_m γ_td γ_ght template_inv op r γ_sy t_id t0,
+          ds_inv N γ_t γ_s γ_m γ_td γ_ght template_inv -∗
+            □ update_helping_protocol N γ_t γ_s γ_td γ_ght -∗
+              thread_vars γ_t γ_ght γ_sy t_id t0 -∗
+                {{{ True }}} 
+                     dsOp (Op_to_val op) #r
+                {{{ res, RET #res; past_lin_witness γ_m op res t0  }}}.
+
+End HINDSIGHT_SPEC.
+
+Module CLIENT_SPEC (DS : DATA_STRUCTURE) (HS: HINDSIGHT_SPEC DS).
+(*   Module DEFS := HINDSIGHT_DEFS DS. *)
+  Import HS DEFS DS.
+
+  Definition dsOp' : val :=
+    λ: "OP" "r",     
+      let: "t_id" := NewProph in
+      let: "p" := NewProph in
+      let: "v" := dsOp "OP" "r" in
+      resolve_proph: "p" to: "v";;
+      "v".
+        
+  (** Proofs *)
+
+  Lemma dsOp'_spec N γ_s γ_t γ_m γ_td γ_ght template_inv op r :
+          ds_inv N γ_t γ_s γ_m γ_td γ_ght template_inv -∗
+              <<< ∀∀ a, dsRep γ_s a >>> 
+                     dsOp' (Op_to_val op) #r @ ↑(cntrN N)
+              <<< ∃∃ a' res, dsRep γ_s a' ∗ ⌜seq_spec op a a' res⌝, RET #res >>>.
+  Proof.
+    iIntros "#HInv" (Φ) "AU". wp_lam. 
+    wp_pure credit:"Hc". wp_pures.
+    wp_apply wp_new_proph1; try done.
+    iIntros (tid vtid)"Htid". wp_pures.
+    wp_apply (typed_proph_wp_new_proph1 resTTypedProph); first done.
+    iIntros (vp p)"Hproph". wp_pures.
+    iApply fupd_wp.
+    iInv "HInv" as (M0 T0 s0) "(>HCntr & >%Habs0 & >Hist & Help & Templ)". 
+    iDestruct "Help" as (R hγt)"(>HR & >Hγt 
+                                & >Domm_hγt & Hstar_reg)".
+    iAssert (▷ (⌜tid ∉ R⌝ 
+            ∗ ([∗ set] t_id ∈ R, Reg N γ_t γ_s γ_ght t_id M0) 
+            ∗ proph1 tid vtid))%I with "[Hstar_reg Htid]" 
+            as "(>% & Hstar_reg & Htid)".
+    { destruct (decide (tid ∈ R)); try done.
+      - iEval (rewrite (big_sepS_elem_of_acc _ (R) tid); 
+                            last by eauto) in "Hstar_reg".
+        iDestruct "Hstar_reg" as "(Hreg & Hstar_reg')".
+        iDestruct "Hreg" as (? ? ? ? ? ? ?)"(H' & _)".
+        iAssert (▷ False)%I with "[H' Htid]" as "HF".
+        iApply (proph1_exclusive tid with "[Htid]"); try done.
+        iNext. iExFalso; try done.
+      - iNext. iFrame. by iPureIntro. }
+    rename H into tid_notin_R.
+    
+    iMod (own_update γ_td (● R) (● (R ∪ {[tid]})) with "[$HR]") as "HR".
+    { apply (auth_update_auth _ _ (R ∪ {[tid]})).
+      apply gset_local_update. set_solver. }
+    iMod (own_update γ_td (● (R ∪ {[tid]})) (● (R ∪ {[tid]}) ⋅ ◯ {[tid]}) 
+              with "[$HR]") as "(HR & #FP_t)".
+    { apply (auth_update_dfrac_alloc _ (R ∪ {[tid]}) ({[tid]})).
+      apply gset_included. clear; set_solver. }
+    
+    iMod (own_alloc (to_frac_agree (1) (M0))) 
+            as (γ_sy)"Hfr_t". { try done. }        
+    iEval (rewrite <-Qp.half_half) in "Hfr_t".      
+    iEval (rewrite (frac_agree_op (1/2) (1/2) _)) in "Hfr_t". 
+    iDestruct "Hfr_t" as "(Hreg_sy1 & Hreg_sy2)".  
+    
+    iDestruct "Domm_hγt" as %Domm_hγt.
+    set (<[ tid := to_agree (T0, γ_sy) ]> hγt) as hγt'.
+    iDestruct (own_update _ _ 
+      (● hγt' ⋅ ◯ {[ tid := to_agree (T0, γ_sy) ]})
+             with "Hγt") as ">Hγt".
+    { apply auth_update_alloc. 
+      rewrite /hγt'.
+      apply alloc_local_update; last done.
+      rewrite <-Domm_hγt in tid_notin_R.
+      by rewrite not_elem_of_dom in tid_notin_R. }
+    iDestruct "Hγt" as "(Hγt & #Hreg_gh)".
+  
+    iMod (own_alloc (Excl ())) as (γ_tk) "Token"; first try done.
+  
+    assert (map_max M0 = T0) as M_max. { admit. }
+    iAssert (own γ_t (◯ (MaxNat T0))) as "HfragT0".
+    { admit. }
+    
+    assert (∀ op c res, Decision (updater_thread op res = true 
+              ∨ (updater_thread op res = false 
+                  ∧ ¬ seq_spec op c c res))) as Hdec.
+    { intros. apply or_dec; try apply updater_thread_dec.
+      apply and_dec; try apply updater_thread_dec.
+      apply neg_seq_spec_dec. }
+      
+    destruct (decide (updater_thread op vp = true 
+      ∨ (updater_thread op vp = false 
+          ∧ ¬ seq_spec op (abs (M0 !!! T0)) (abs (M0 !!! T0)) vp))) 
+      as [Hcase1 | Hcase2]; clear Hdec.
+    - iMod (inv_alloc (threadN N) _
+              (∃ M T, State γ_sy γ_tk (au N γ_s op Φ) Φ M T op vp T0) 
+                                    with "[AU Hc Hreg_sy1]") as "#HthInv".
+      { iNext. iExists M0, T0. iFrame "Hreg_sy1".
+        iSplitR. { by iPureIntro. }
+        iLeft. unfold Pending. iFrame.
+        unfold past_lin.
+        destruct Hcase1 as [H' | H'].
+        - rewrite H'. iIntros "%Hpast". 
+          destruct Hpast as [t [H'' _]]. lia.
+        - destruct H' as [H1' H2'].
+          rewrite H1'. iIntros "%Hpast". 
+          destruct Hpast as [t [H' Hss]].
+          assert (t = T0) as -> by lia. contradiction. }
+
+      iModIntro. iSplitR "Hproph Token". iNext.
+      iExists M0, T0, s0. iFrame "∗%".
+      iExists (R ∪ {[tid]}), hγt'. iFrame.
+      iSplitR. iPureIntro. subst hγt'.
+      apply leibniz_equiv. rewrite dom_insert.
+      rewrite Domm_hγt. clear; set_solver.
+      rewrite (big_sepS_delete _ (R ∪ {[tid]}) tid); last by set_solver.
+      iSplitR "Hstar_reg". unfold Reg.
+      iExists γ_tk, γ_sy, Φ, op, vp, T0, vtid. iFrame "∗#".
+      assert ((R ∪ {[tid]}) ∖ {[tid]} = R) as H' 
+                  by (clear -tid_notin_R; set_solver).
+      by rewrite H'.
+      
+      iModIntro. wp_bind (dsOp _ _)%E.
+      
+      iAssert (update_helping_protocol N γ_t γ_s γ_td γ_ght)%I as "Upd_help".
+      { admit. }
+      iAssert (thread_vars γ_t γ_ght γ_sy tid T0)%I as "#Thr_vars".
+      { iFrame "#". }
+
+      wp_apply dsOp_spec; try done.
+      iIntros (res)"HpastW".
+      wp_pures.
+      wp_apply ((typed_proph_wp_resolve1 resTTypedProph 
+                  _ _ _ _ _ _ _ (res))
+        with "Hproph"); try done.
+      { unfold typed_proph_from_val; simpl. by rewrite resT_proph_resolve. }  
+      wp_pures. iModIntro. iIntros "%vp_eq_res". subst vp.
+       
+      iApply fupd_wp.
+      
+      iInv "HthInv" as (M1_th T1_th)"(>Hth_sy & >% & Hth_or)".
+      iInv "HInv" as (M1 T1 s1) "(>HCntr & >%Habs1 & >Hist & Help & Templ)".
+      iDestruct "Help" as (R1 hγt1)"(>HR & >Hγt 
+                                  & >Domm_hγt & Hstar_reg)".
+      
+      iAssert (⌜tid ∈ R1⌝)%I as "%".
+      { iPoseProof (own_valid_2 _ _ _ with "[$HR] [$FP_t]") as "H'".
+        iDestruct "H'" as %H'.
+        apply auth_both_valid_discrete in H'.
+        destruct H' as [H' _].
+        apply gset_included in H'.
+        iPureIntro. set_solver. }
+      rename H into tid_in_R1.
+      
+      iAssert (▷ (⌜M1_th = M1⌝ ∗ ⌜T1_th = T1⌝ 
+               ∗ ([∗ set] t_id ∈ R1, Reg N γ_t γ_s γ_ght t_id M1)
+               ∗ own (γ_sy) (to_frac_agree (1 / 2) M1_th) ))%I
+                with "[Hstar_reg Hth_sy]" as "(>% & >% & Hstar_reg & >Hth_sy)". 
+      { 
+        iEval (rewrite (big_sepS_elem_of_acc _ (R1) tid); 
+                                last by eauto) in "Hstar_reg".
+        iDestruct "Hstar_reg" as "(Hreg_t & Hstar_reg')".
+        iDestruct "Hreg_t" as (γ_tk' γ_sy' Q' op' vp' t0' vtid')
+                          "(Hreg_proph & >Hreg_gh' & >Hreg_sy & Ht_reg')".
+
+        iDestruct "Hreg_gh'" as "(Hreg_gh' & #?)".
+        iCombine "Hreg_gh" "Hreg_gh'" as "H".
+        iPoseProof (own_valid with "H") as "Valid".
+        iDestruct "Valid" as %Valid.
+        rewrite auth_frag_valid in Valid.
+        apply singleton_valid in Valid.
+        apply to_agree_op_inv in Valid.
+        apply leibniz_equiv in Valid.
+        injection Valid; intros <- <-.
+                  
+        iAssert (⌜M1_th = M1 ∧ T1_th = T1⌝)%I as "(% & %)".
+        { iPoseProof (own_valid_2 _ _ _ with "[$Hth_sy] [$Hreg_sy]") 
+              as "V_M".
+          iDestruct "V_M" as %V_M.
+          apply frac_agree_op_valid in V_M. destruct V_M as [_ V_M].
+          iPureIntro. split; first by apply leibniz_equiv. admit. } 
+        subst M1_th T1_th.
+          
+        iSplitR. { by iPureIntro. } 
+        iSplitR. iNext; by iPureIntro.
+        iSplitR "Hth_sy". iApply "Hstar_reg'".
+        iNext. iExists γ_tk', γ_sy, Q', op', vp', T0, vtid'.
+        iFrame "∗#". by iNext. 
+      } subst M1_th T1_th.
+      
+      iEval (unfold past_lin_witness) in "HpastW".
+      (* iEval (rewrite Upd_thr) in "HpastW".*)
+
+      iDestruct "Hth_or" as "[Hth_or | Hth_or]".
+      { iDestruct "Hth_or" as "(AU & Hc & >%HPending)".
+        destruct (decide (updater_thread op res = true))
+          as [Hdec | Hdec]. 
+        - rewrite Hdec. rewrite Hdec in HPending.
+          iExFalso. admit. 
+        - destruct (decide (updater_thread op res = false)) as [Hdec' | Hdec'].
+          + rewrite Hdec'. rewrite Hdec' in HPending. 
+            iExFalso. admit.
+          + admit. }  
+      
+      iDestruct "Hth_or" as "(Hth_or & Hpast)".  
+      iDestruct "Hth_or" as "[Hth_or | >Hth_or]"; last first.
+      { iPoseProof (own_valid_2 _ _ _ with "[$Token] [$Hth_or]") as "%".
+        exfalso; try done. }
+        
+      iModIntro. iSplitR "Hth_or Hth_sy Token Hpast".
+      iExists M1, T1, s1; iFrame "∗%".
+      iNext. iExists R1, hγt1; iFrame.     
+
+      iModIntro. iSplitL "Token Hth_sy Hpast".
+      iNext. iExists M1, T1. iFrame "Hth_sy". 
+      iSplitR. by iPureIntro. iRight. iFrame "∗%".
+      by subst T1.
+      
+      iModIntro. by wp_pures.
+    - assert (updater_thread op vp = false 
+        ∧ seq_spec op (abs (M0 !!! T0)) (abs (M0 !!! T0)) vp) as [Upd_thr Hss]. 
+      { clear -Hcase2. destruct (updater_thread op vp); split.
+        - exfalso; apply Hcase2. left; try done.
+        - exfalso; apply Hcase2. left; try done. 
+        - done. 
+        - assert (Decision (seq_spec op (abs (M0 !!! T0)) (abs (M0 !!! T0)) vp)) as H'.
+          { apply seq_spec_dec. }
+          destruct (decide (seq_spec op (abs (M0 !!! T0)) (abs (M0 !!! T0)) vp));
+            try done. 
+          exfalso. apply Hcase2. right.
+          split; try done. } 
+      iMod "AU" as (c) "[Cntr [_ Hcomm]]".
+      iAssert (⌜c = abs s0⌝)%I as "%". { admit. } subst c. 
+      iSpecialize ("Hcomm" $! (abs s0) vp). 
+      iMod ("Hcomm" with "[Cntr]") as "HΦ".
+      { iFrame. rewrite Habs0 in Hss. by iPureIntro. }
+   
+      iAssert (past_lin M0 T0 op vp T0)%I as "Hpast".
+      { iPureIntro. rewrite Upd_thr. exists T0.
+        split; try done. }
+        
+      iMod (inv_alloc (threadN N) _
+            (∃ M T, State γ_sy γ_tk (au N γ_s op Φ) Φ M T op vp T0) 
+                                  with "[Hreg_sy1 Token]") as "#HthInv".
+      { iNext. iExists M0, T0. iFrame "Hreg_sy1".
+        iSplitR. by iPureIntro.
+        iRight. unfold Done. iFrame "Hpast".
+        by iRight. }
+      
+      iAssert (update_helping_protocol N γ_t γ_s γ_td γ_ght)%I as "Upd_help".
+      { admit. }
+      iAssert (thread_vars γ_t γ_ght γ_sy tid T0)%I as "#Thr_vars".
+      { iFrame "#". }
+  
+      
+      iModIntro. iSplitR "Hproph HΦ". iNext.
+      iExists M0, T0, s0.  iFrame "∗%".
+      iExists (R ∪ {[tid]}), hγt'. iFrame.
+      iSplitR. iPureIntro. subst hγt'.
+      apply leibniz_equiv. rewrite dom_insert.
+      rewrite Domm_hγt. clear; set_solver.
+      rewrite (big_sepS_delete _ (R ∪ {[tid]}) tid); last by set_solver.
+      iSplitR "Hstar_reg". unfold Reg.
+      iExists γ_tk, γ_sy, Φ, op, vp, T0, vtid. iFrame "∗#".
+      assert ((R ∪ {[tid]}) ∖ {[tid]} = R) as H' 
+                by (clear -tid_notin_R; set_solver).
+      by rewrite H'.  
+        
+      iModIntro.
+      wp_apply dsOp_spec; try done.
+      iIntros (res)"HpastW". wp_pures.
+      wp_apply ((typed_proph_wp_resolve1 resTTypedProph 
+                  _ _ _ _ _ _ _ (res))
+        with "Hproph"); try done.
+      { unfold typed_proph_from_val; simpl. by rewrite resT_proph_resolve. }    
+      wp_pures. iModIntro. iIntros "->".
+      wp_pures. iModIntro. done. 
+    
+  Admitted.
+  
+End CLIENT_SPEC.  
+  
+  
+  
+  
+  
+  
+  
+  
+  
+  
+  
+  
+  
